```
<헷갈렸던점✨>
(lx - x[idx])^2 + (ly- y[idx])^2
=>
abs(lx - x[idx]) + abs(ly- y[idx]) 
이렇게 고쳤더니 정답
```
```python
def solution(numbers, hand):
    x=[0,1,2,0,1,2,0,1,2,0,1,2]
    y = [0,0,0,1,1,1,2,2,2,3,3,3]
    graph = [1,2,3,4,5,6,7,8,9,'*',0,'#']
    lx , rx,ly, ry= 0,2,3,3
    answer=''
    for i in numbers:
        idx= graph.index(i)
        if i in [2,5,8,0]:
            ld = abs(lx - x[idx]) + abs(ly- y[idx])
            rd = abs(rx - x[idx]) + abs(ry- y[idx])
            if ld>rd:
                answer+='R'
                rx,ry = x[idx],y[idx]
            elif ld<rd:
                answer+='L'
                lx,ly = x[idx],y[idx]
            else:
                if hand=='right':
                    answer+='R'
                    rx,ry = x[idx],y[idx]
                else: 
                    answer+='L'
                    lx,ly = x[idx],y[idx]
        elif i in [1,4,7]:
            answer+='L'
            lx,ly = x[idx],y[idx]
        else:
            answer+='R'
            rx,ry = x[idx],y[idx]
            
    return answer
```